---
layout: default
title: "Corrigé de l’exercice"
---
# Exercice 1 — Sujet A

## Corrigé de l'exercice 1
1. On a : $\begin{aligned} \dfrac{(4+h)^2-6(4+h)-4^2+24}{h}&=\dfrac{16+8h+h^2-24-6h-16+24}{h}\\
&=\dfrac{h^2+2h}{h}\\&=\dfrac{h(h+2)}{h}\\&=h+2\end{aligned}$

2. On a $$\begin{aligned}\dfrac{f(4+h)-f(4)}{h}&=\dfrac{(4+h)^2-6(4+h)-(4^2-6\times 4)}{h}\\&=\dfrac{(4+h)^2-6(4+h)-4^2+24}{h}\\ &=h+2
\end{aligned}$$. 
De plus $\displaystyle\lim_{h\mapsto 0}  (h+2)=2$, on en déduit que $f$ est dérivable en $4$ et on a $f'(4)=2$. 
---

<script src="https://cdn.jsdelivr.net/npm/mathjax@3/es5/tex-mml-chtml.js"></script>
