---
layout: default
title: "Corrigé de l’exercice"
---
## Corrigé de l'exercice 2

On a : $g(x)=\sqrt{x+9}$.
1. $(\sqrt{9+h}-3)(\sqrt{9+h}+3)=(\sqrt{9+h})^2-3^2=9+h-9=h$
2. 
$ \frac{g(0+h)-g(0)}{h}=\frac{\sqrt{h+9}-3}{h}
=\dfrac{(\sqrt{h+9}-3)(\sqrt{h+9}+3)}{h(\sqrt{h+9}+3)}
=\dfrac{h}{h(\sqrt{h+9}+3))}
=\dfrac{1}{\sqrt{h+9}+3}$



3. On a : $$ \begin{aligned} 
\lim_{h\mapsto 0} \dfrac{g(0+h)-g(0)}{h} 
& =\lim_{h\mapsto 0} \dfrac{1}{\sqrt{h+9}+3} \\
&=\dfrac{1}{\sqrt{0+9}+3}\\
&=\dfrac{1}{6}
\end{aligned}
$$

---

<script src="https://cdn.jsdelivr.net/npm/mathjax@3/es5/tex-mml-chtml.js"></script>
